src/Std/Data/DHashMap/Raw.lean
@@ -705,6 +705,10 @@ theorem WF.Const.unitOfList [BEq α] [Hashable α] {l : List α} :
     (Const.unitOfList l : Raw α (fun _ => Unit)).WF :=
   Const.insertManyIfNewUnit WF.empty
 
+theorem WF.union [BEq α] [Hashable α] {m₁ m₂ : Raw α β} (h₁ : m₁.WF) (h₂ : m₂.WF) : (m₁.union m₂ : Raw α β).WF := by
+  simp [Std.DHashMap.Raw.union, h₁.size_buckets_pos, h₂.size_buckets_pos]
+  sorry
+
 end WF
 
 end Raw
